stronger soundness lemma

CrIdentifiers.v
@@ -3,6 +3,7 @@ From MyProject Require Import Integers.
 From MyProject Require Import MyInts.
 From MyProject Require Import InitStatus.
 From Stdlib Require Import ZArith.
+From Stdlib Require Import PArith.BinPos.
 From Stdlib Require Import Bool.
 From Stdlib Require Import List.
 Import ListNotations.
@@ -22,20 +23,36 @@ Definition parser_state_equal (p1 p2 : ParserState) :=
             | ParserStateCtr xid, ParserStateCtr yid => Pos.eqb xid yid
     end.
 
-(* Do the same thing as parser_state_equal for ModuleName *)
 Definition module_name_equal (m1 m2 : ModuleName) :=
     match m1, m2 with
             | ModuleNameCtr xid, ModuleNameCtr yid => Pos.eqb xid yid
     end.
 
-(* Do the same thing as parser_state_equal for FunctionName *)
 Definition function_name_equal (f1 f2 : FunctionName) :=
     match f1, f2 with
             | FunctionNameCtr xid, FunctionNameCtr yid => Pos.eqb xid yid
     end.
 
-(* Do the same thing as parser_state_equal for ConnectionName *)
 Definition connection_name_equal (c1 c2 : ConnectionName) :=
     match c1, c2 with
             | ConnectionNameCtr xid, ConnectionNameCtr yid => Pos.eqb xid yid
     end.
+
+(* Decidable equality for the varlike identifiers, derived from positive equality. *)
+Definition header_eq_dec : forall x y : Header, {x = y} + {x <> y}.
+Proof.
+  intros [a] [b]. destruct (Pos.eq_dec a b);
+    [left; subst; reflexivity | right; intro Heq; inversion Heq; contradiction].
+Defined.
+
+Definition state_eq_dec : forall x y : State, {x = y} + {x <> y}.
+Proof.
+  intros [a] [b]. destruct (Pos.eq_dec a b);
+    [left; subst; reflexivity | right; intro Heq; inversion Heq; contradiction].
+Defined.
+
+Definition ctrl_eq_dec : forall x y : Ctrl, {x = y} + {x <> y}.
+Proof.
+  intros [a] [b]. destruct (Pos.eq_dec a b);
+    [left; subst; reflexivity | right; intro Heq; inversion Heq; contradiction].
+Defined.
